otbn_model/code/modexp_var_lemmas.dfy
@@ -74,43 +74,43 @@ module modexp_var_lemmas {
         a: nat,
         sig: nat,
         i: nat,
-        key: pub_key)
-        requires key.m != 0;
+        rsa: rsa_params)
+        requires rsa.m != 0;
     {
-        cong(a, power(sig, power(2, i)) * key.R, key.m)
+        cong(a, power(sig, power(2, i)) * rsa.R, rsa.m)
     }
 
     lemma modexp_var_inv_lemma_0(
         a_slice: seq<uint256>,
         rr: seq<uint256>,
         sig: seq<uint256>,
-        key: pub_key)
+        rsa: rsa_params)
 
-    requires montmul_inv(a_slice, rr, NUM_WORDS, sig, key);
-    requires to_nat(rr) == key.RR;
-    ensures modexp_var_inv(to_nat(a_slice), to_nat(sig), 0, key);
+    requires montmul_inv(a_slice, rr, NUM_WORDS, sig, rsa);
+    requires to_nat(rr) == rsa.RR;
+    ensures modexp_var_inv(to_nat(a_slice), to_nat(sig), 0, rsa);
     {
-        var m := key.m;
+        var m := rsa.m;
         var a := to_nat(a_slice);
         var s := to_nat(sig);
 
-        assert cong(key.RR * key.R_INV, key.R, m) by {
-            assert cong(key.R * key.R * key.R_INV, key.R, m) by {
-                r_r_inv_cancel_lemma(key.R, key);
+        assert cong(rsa.RR * rsa.R_INV, rsa.R, m) by {
+            assert cong(rsa.R * rsa.R * rsa.R_INV, rsa.R, m) by {
+                r_r_inv_cancel_lemma(rsa.R, rsa);
             }
-            assert cong(key.RR * key.R_INV, key.R * key.R * key.R_INV, m) by {
-                assert cong(key.RR, key.R * key.R, m);
-                cong_mul_lemma_1(key.RR, key.R * key.R, key.R_INV, m);
+            assert cong(rsa.RR * rsa.R_INV, rsa.R * rsa.R * rsa.R_INV, m) by {
+                assert cong(rsa.RR, rsa.R * rsa.R, m);
+                cong_mul_lemma_1(rsa.RR, rsa.R * rsa.R, rsa.R_INV, m);
             }
             reveal cong();
         }
 
-        assert cong(a, s * key.R, m) by {
-            assert cong(key.RR * key.R_INV * s, key.R * s, m) by {
-                cong_mul_lemma_1(key.RR * key.R_INV, key.R, s, m);
+        assert cong(a, s * rsa.R, m) by {
+            assert cong(rsa.RR * rsa.R_INV * s, rsa.R * s, m) by {
+                cong_mul_lemma_1(rsa.RR * rsa.R_INV, rsa.R, s, m);
             }
-            assert cong(a, key.RR * key.R_INV * s, m) by {
-                montmul_inv_lemma_1(a_slice, rr, sig, key);
+            assert cong(a, rsa.RR * rsa.R_INV * s, m) by {
+                montmul_inv_lemma_1(a_slice, rr, sig, rsa);
             }
             reveal cong();
         }
@@ -123,39 +123,39 @@ module modexp_var_lemmas {
         next_a_slice: seq<uint256>,
         sig: nat,
         i: nat,
-        key: pub_key)
+        rsa: rsa_params)
 
-        requires montmul_inv(next_a_slice, a_slice, NUM_WORDS, a_slice, key);
-        requires modexp_var_inv(to_nat(a_slice), sig, i, key);
-        ensures modexp_var_inv(to_nat(next_a_slice), sig, i + 1, key);
+        requires montmul_inv(next_a_slice, a_slice, NUM_WORDS, a_slice, rsa);
+        requires modexp_var_inv(to_nat(a_slice), sig, i, rsa);
+        ensures modexp_var_inv(to_nat(next_a_slice), sig, i + 1, rsa);
     {
-        var m := key.m;
+        var m := rsa.m;
         var a := to_nat(a_slice);
         var next_a := to_nat(next_a_slice);
-        var next_goal := power(sig, power(2, i + 1)) * key.R;
+        var next_goal := power(sig, power(2, i + 1)) * rsa.R;
 
-        assert cong(a, power(sig, power(2, i)) * key.R, m);
+        assert cong(a, power(sig, power(2, i)) * rsa.R, m);
         
         calc ==> {
-            cong(a, power(sig, power(2, i)) * key.R, m);
-                { cong_mul_lemma_2(a, power(sig, power(2, i)) * key.R, 
-                    a, power(sig, power(2, i)) * key.R, m); }
-            cong(a * a, power(sig, power(2, i)) * key.R * power(sig, power(2, i)) * key.R, m);
+            cong(a, power(sig, power(2, i)) * rsa.R, m);
+                { cong_mul_lemma_2(a, power(sig, power(2, i)) * rsa.R, 
+                    a, power(sig, power(2, i)) * rsa.R, m); }
+            cong(a * a, power(sig, power(2, i)) * rsa.R * power(sig, power(2, i)) * rsa.R, m);
                 { power_same_base_lemma(sig, power(2, i), power(2, i)); }
-            cong(a * a, power(sig, power(2, i) + power(2, i)) * key.R * key.R, m);
-            cong(a * a, power(sig, power(2, i) * 2) * key.R * key.R, m);
+            cong(a * a, power(sig, power(2, i) + power(2, i)) * rsa.R * rsa.R, m);
+            cong(a * a, power(sig, power(2, i) * 2) * rsa.R * rsa.R, m);
                 { power_add_one_lemma(2, i); }
-            cong(a * a, next_goal * key.R, m);
-                { cong_mul_lemma_1(a * a, next_goal * key.R, key.R_INV, m); }
-            cong(a * a * key.R_INV, next_goal * key.R * key.R_INV, m);
+            cong(a * a, next_goal * rsa.R, m);
+                { cong_mul_lemma_1(a * a, next_goal * rsa.R, rsa.R_INV, m); }
+            cong(a * a * rsa.R_INV, next_goal * rsa.R * rsa.R_INV, m);
                 {
-                    assert cong(next_a, a * a * key.R_INV, m) by {
-                        montmul_inv_lemma_1(next_a_slice, a_slice, a_slice, key);
+                    assert cong(next_a, a * a * rsa.R_INV, m) by {
+                        montmul_inv_lemma_1(next_a_slice, a_slice, a_slice, rsa);
                     }
-                    cong_trans_lemma(next_a, a * a * key.R_INV, next_goal * key.R * key.R_INV, m);
+                    cong_trans_lemma(next_a, a * a * rsa.R_INV, next_goal * rsa.R * rsa.R_INV, m);
                 }
-            cong(next_a, next_goal * key.R_INV * key.R, m);
-                { r_r_inv_cancel_lemma_2(next_a, next_goal, key); }
+            cong(next_a, next_goal * rsa.R_INV * rsa.R, m);
+                { r_r_inv_cancel_lemma_2(next_a, next_goal, rsa); }
             cong(next_a, next_goal, m);
         }
 
@@ -165,42 +165,42 @@ module modexp_var_lemmas {
         a_slice: seq<uint256>,
         next_a_slice: seq<uint256>,
         sig: seq<uint256>,
-        key: pub_key)
+        rsa: rsa_params)
 
-        requires montmul_inv(next_a_slice, a_slice, NUM_WORDS, sig, key);
-        requires modexp_var_inv(to_nat(a_slice), to_nat(sig), key.e', key);
-        ensures cong(to_nat(next_a_slice), power(to_nat(sig), key.e), key.m);
+        requires montmul_inv(next_a_slice, a_slice, NUM_WORDS, sig, rsa);
+        requires modexp_var_inv(to_nat(a_slice), to_nat(sig), rsa.e', rsa);
+        ensures cong(to_nat(next_a_slice), power(to_nat(sig), rsa.e), rsa.m);
     {
-        var m := key.m;
+        var m := rsa.m;
         var a := to_nat(a_slice);
         var next_a := to_nat(next_a_slice);
         var s := to_nat(sig);
-        var cur := power(s, power(2, key.e'));
+        var cur := power(s, power(2, rsa.e'));
 
-        assert cong(a, cur * key.R, m);
+        assert cong(a, cur * rsa.R, m);
 
         calc ==> {
-            cong(a, cur * key.R, m);
-                { cong_mul_lemma_1(a, cur * key.R, s * key.R_INV, m); }
-            cong(a * (s * key.R_INV), (cur * key.R) * (s * key.R_INV), m);
+            cong(a, cur * rsa.R, m);
+                { cong_mul_lemma_1(a, cur * rsa.R, s * rsa.R_INV, m); }
+            cong(a * (s * rsa.R_INV), (cur * rsa.R) * (s * rsa.R_INV), m);
                 {
-                    assert a * (s * key.R_INV) == a * s * key.R_INV;
-                    assert (cur * key.R) * (s * key.R_INV) == cur * key.R * s * key.R_INV;
+                    assert a * (s * rsa.R_INV) == a * s * rsa.R_INV;
+                    assert (cur * rsa.R) * (s * rsa.R_INV) == cur * rsa.R * s * rsa.R_INV;
                 }
-            cong(a * s * key.R_INV, cur * key.R * s * key.R_INV, m);
+            cong(a * s * rsa.R_INV, cur * rsa.R * s * rsa.R_INV, m);
                 {
-                    assert cong(next_a, a * s * key.R_INV, m) by {
-                        montmul_inv_lemma_1(next_a_slice, a_slice, sig, key);
+                    assert cong(next_a, a * s * rsa.R_INV, m) by {
+                        montmul_inv_lemma_1(next_a_slice, a_slice, sig, rsa);
                     }
-                    cong_trans_lemma(next_a, a * s * key.R_INV, cur * key.R * s * key.R_INV, m);
+                    cong_trans_lemma(next_a, a * s * rsa.R_INV, cur * rsa.R * s * rsa.R_INV, m);
                 }
-            cong(next_a, cur * key.R * s * key.R_INV, m);
-                { r_r_inv_cancel_lemma_2(next_a, cur * s, key); }
+            cong(next_a, cur * rsa.R * s * rsa.R_INV, m);
+                { r_r_inv_cancel_lemma_2(next_a, cur * s, rsa); }
             cong(next_a, cur * s, m);
-                { power_add_one_lemma(s, power(2, key.e')); }
-            cong(next_a, power(s, power(2, key.e') + 1), m);
-            cong(next_a, power(s, key.e), m);
-            cong(to_nat(next_a_slice), power(to_nat(sig), key.e), m);
+                { power_add_one_lemma(s, power(2, rsa.e')); }
+            cong(next_a, power(s, power(2, rsa.e') + 1), m);
+            cong(next_a, power(s, rsa.e), m);
+            cong(to_nat(next_a_slice), power(to_nat(sig), rsa.e), m);
         }
 
     }
@@ -216,33 +216,33 @@ module modexp_var_lemmas {
         adjusted_val: nat,
         carry: bool,
         sig: nat,
-        key: pub_key)
+        rsa: rsa_params)
 
-    requires pub_key_inv(key);
-    requires raw_val < sig + key.m;
-    requires cong(raw_val, power(sig, key.e), key.m);
-    requires carry ==> raw_val < key.m;
-    requires !carry ==> raw_val - key.m == adjusted_val;
+    requires rsa_params_inv(rsa);
+    requires raw_val < sig + rsa.m;
+    requires cong(raw_val, power(sig, rsa.e), rsa.m);
+    requires carry ==> raw_val < rsa.m;
+    requires !carry ==> raw_val - rsa.m == adjusted_val;
 
-    ensures carry ==> raw_val == power(sig, key.e) % key.m;
-    ensures !carry ==> adjusted_val == power(sig, key.e) % key.m;
+    ensures carry ==> raw_val == power(sig, rsa.e) % rsa.m;
+    ensures !carry ==> adjusted_val == power(sig, rsa.e) % rsa.m;
     {
         if carry {
-            cong_remainder_lemma(raw_val, power(sig, key.e), key.m);
-            assert raw_val == power(sig, key.e) % key.m;
+            cong_remainder_lemma(raw_val, power(sig, rsa.e), rsa.m);
+            assert raw_val == power(sig, rsa.e) % rsa.m;
         } else {
-            assume sig < key.m; // TODO: fix this
+            assume sig < rsa.m; // TODO: fix this
             calc ==> {
                 true;
-                    { cong_add_lemma_3(raw_val, -(key.m as int), key.m); }
-                cong(raw_val, adjusted_val, key.m);
+                    { cong_add_lemma_3(raw_val, -(rsa.m as int), rsa.m); }
+                cong(raw_val, adjusted_val, rsa.m);
                     {
-                        cong_trans_lemma(adjusted_val, raw_val, power(sig, key.e), key.m);
+                        cong_trans_lemma(adjusted_val, raw_val, power(sig, rsa.e), rsa.m);
                     }
-                cong(adjusted_val, power(sig, key.e), key.m);
+                cong(adjusted_val, power(sig, rsa.e), rsa.m);
             }
 
-            cong_remainder_lemma(adjusted_val, power(sig, key.e), key.m);
+            cong_remainder_lemma(adjusted_val, power(sig, rsa.e), rsa.m);
         }
     }
 }
