otbn_model/code/montmul_lemmas.dfy
@@ -14,37 +14,37 @@ module montmul_lemmas {
         x: seq<uint256>, 
         i: nat,
         y: seq<uint256>, 
-        key: pub_key)
+        rsa: rsa_params)
 
         requires |a| == |x| == |y| == NUM_WORDS;
         requires to_nat(a) == 0;
-        requires pub_key_inv(key);
+        requires rsa_params_inv(rsa);
         requires i == 0;
         
-        ensures montmul_inv(a, x, i, y, key);
+        ensures montmul_inv(a, x, i, y, rsa);
     {
         assert to_nat(x[..i]) == 0 by {
             reveal to_nat();
         }
         reveal cong();
-        assert montmul_inv(a, x, i, y, key);
+        assert montmul_inv(a, x, i, y, rsa);
     }
 
-    lemma r_r_inv_cancel_lemma(a: nat, key: pub_key)
-        requires pub_key_inv(key);
-        ensures cong(a * key.R_INV * key.R, a, key.m);
+    lemma r_r_inv_cancel_lemma(a: nat, rsa: rsa_params)
+        requires rsa_params_inv(rsa);
+        ensures cong(a * rsa.R_INV * rsa.R, a, rsa.m);
     {
-        assert cong(key.R_INV * key.R, 1, key.m);
-        cong_mul_lemma_1(key.R_INV * key.R, 1, a, key.m);
+        assert cong(rsa.R_INV * rsa.R, 1, rsa.m);
+        cong_mul_lemma_1(rsa.R_INV * rsa.R, 1, a, rsa.m);
     }
     
-    lemma r_r_inv_cancel_lemma_2(a: nat, b : nat, key: pub_key)
-        requires pub_key_inv(key);
-        requires cong(a, b * key.R_INV * key.R, key.m);
-        ensures cong(a, b, key.m);
+    lemma r_r_inv_cancel_lemma_2(a: nat, b : nat, rsa: rsa_params)
+        requires rsa_params_inv(rsa);
+        requires cong(a, b * rsa.R_INV * rsa.R, rsa.m);
+        ensures cong(a, b, rsa.m);
     {
-        assert cong(b * key.R_INV * key.R, b, key.m) by {
-            r_r_inv_cancel_lemma(b, key);
+        assert cong(b * rsa.R_INV * rsa.R, b, rsa.m) by {
+            r_r_inv_cancel_lemma(b, rsa);
         }
         reveal cong();
     }
@@ -52,25 +52,25 @@ module montmul_lemmas {
     lemma montmul_inv_lemma_1(a_slice: seq<uint256>,
         x: seq<uint256>,
         y: seq<uint256>,
-        key: pub_key)
+        rsa: rsa_params)
     
-        requires montmul_inv(a_slice, x, NUM_WORDS, y, key);
-        ensures cong(to_nat(a_slice), to_nat(x) * to_nat(y) * key.R_INV, key.m);
+        requires montmul_inv(a_slice, x, NUM_WORDS, y, rsa);
+        ensures cong(to_nat(a_slice), to_nat(x) * to_nat(y) * rsa.R_INV, rsa.m);
     {
-        var m := key.m;
+        var m := rsa.m;
         var a := to_nat(a_slice);
         assert x[..NUM_WORDS] == x;
 
         calc ==> {
-            cong(a * key.R, to_nat(x) * to_nat(y), m);
-                { cong_mul_lemma_1(a * key.R, to_nat(x) * to_nat(y), key.R_INV, m); }
-            cong(a * key.R * key.R_INV, to_nat(x) * to_nat(y) * key.R_INV, m);
+            cong(a * rsa.R, to_nat(x) * to_nat(y), m);
+                { cong_mul_lemma_1(a * rsa.R, to_nat(x) * to_nat(y), rsa.R_INV, m); }
+            cong(a * rsa.R * rsa.R_INV, to_nat(x) * to_nat(y) * rsa.R_INV, m);
                 { reveal cong(); }
-            cong(to_nat(x) * to_nat(y) * key.R_INV, a * key.R * key.R_INV, m);
-                { r_r_inv_cancel_lemma_2(to_nat(x) * to_nat(y) * key.R_INV, a, key); }
-            cong(to_nat(x) * to_nat(y) * key.R_INV, a, m);
+            cong(to_nat(x) * to_nat(y) * rsa.R_INV, a * rsa.R * rsa.R_INV, m);
+                { r_r_inv_cancel_lemma_2(to_nat(x) * to_nat(y) * rsa.R_INV, a, rsa); }
+            cong(to_nat(x) * to_nat(y) * rsa.R_INV, a, m);
                 { reveal cong(); }
-            cong(a, to_nat(x) * to_nat(y) * key.R_INV, m);
+            cong(a, to_nat(x) * to_nat(y) * rsa.R_INV, m);
         }
     }
 }
